fstar/MLS.TreeSync.Symbolic.API.fst
@@ -4,15 +4,19 @@ open GlobalRuntimeLib
 open LabeledRuntimeAPI
 open MLS.NetworkTypes
 open MLS.TreeSync.NetworkTypes
+open MLS.TreeSync.Types
 open MLS.TreeSync.Invariants.AuthService
 open MLS.TreeSync.API
 open MLS.Symbolic
 open MLS.TreeSync.Symbolic.API.GroupManager
+open MLS.TreeSync.Symbolic.API.KeyPackageManager
 open MLS.TreeSync.Symbolic.API.Sessions
 open MLS.TreeSync.Symbolic.API.HasPreInvariant
 open MLS.TreeSync.Symbolic.SignatureGuarantees
 open MLS.TreeSync.Symbolic.AuthServiceCache
 open MLS.TreeSync.Symbolic.IsValid
+
+#set-options "--fuel 0 --ifuel 0"
 
 val guard: pr:preds -> b:bool -> LCrypto unit pr
   (requires fun t0 -> True)
@@ -21,6 +25,7 @@ let guard pr b =
   if b then ()
   else error "guard failed"
 
+#push-options "--ifuel 1"
 val extract_result: #a:Type -> pr:preds -> MLS.Result.result a -> LCrypto a pr
   (requires fun t0 -> True)
   (ensures fun t0 _ t1 -> t1 == t0)
@@ -29,12 +34,14 @@ let extract_result #a pr x =
   | MLS.Result.Success y -> y
   | MLS.Result.InternalError s -> error "extract_result: internal error '" ^ s ^ "'"
   | MLS.Result.ProtocolError s -> error "extract_result: protocol error '" ^ s ^ "'"
+#pop-options
 
 val has_treesync_invariants: treekem_types dy_bytes -> preds -> prop
 let has_treesync_invariants tkt pr =
   has_treesync_public_state_invariant tkt pr /\
   has_treesync_private_state_invariant pr /\
   has_group_manager_invariant pr /\
+  has_key_package_manager_invariant tkt pr /\
   has_as_cache_invariant pr
 
 val get_token_for:
@@ -52,9 +59,85 @@ let get_token_for pr p as_session (verification_key, credential) =
   guard pr (usg = "MLS.LeafSignKey");
   { who; time; }
 
-//TODO create
+#push-options "--fuel 1 --ifuel 1"
+val get_tokens_for:
+  pr:preds -> p:principal -> as_session:nat ->
+  inps:list (option (as_input dy_bytes)) ->
+  LCrypto (list (option dy_as_token)) pr
+  (requires fun t0 -> has_as_cache_invariant pr)
+  (ensures fun t0 tokens t1 ->
+    List.Tot.length tokens == List.Tot.length inps /\
+    (forall i.
+      match (List.Tot.index inps i), (List.Tot.index tokens i) with
+      | None, None -> True
+      | Some inp, Some token -> (dy_asp pr.global_usage (trace_len t0)).credential_ok inp token
+      | _, _ -> False
+    ) /\
+    t1 == t0
+  )
+let rec get_tokens_for pr p as_session inps =
+  let now = global_timestamp () in
+  match inps with
+  | [] -> []
+  | inp_head::inps_tail ->
+    let token_head =
+      match inp_head with
+      | Some inp -> Some (get_token_for pr p as_session inp)
+      | None -> None
+    in
+    let tokens_tail = get_tokens_for pr p as_session inps_tail in
+    let tokens = token_head::tokens_tail in
+    // An assert is needed to trigger the `forall`
+    assert(forall i. i <> 0 ==> List.Tot.index inps i == List.Tot.index inps_tail (i-1));
+    tokens
+#pop-options
 
-//TODO welcome
+val create:
+  #tkt:treekem_types dy_bytes ->
+  pr:preds -> p:principal -> as_session:nat -> gmgr_session:nat ->
+  group_id:mls_bytes dy_bytes -> ln:leaf_node_nt dy_bytes tkt -> secret_session:nat ->
+  LCrypto unit pr
+  (requires fun t0 ->
+    is_publishable pr.global_usage (trace_len t0) group_id /\
+    value_has_pre (is_publishable pr.global_usage (trace_len t0)) ln /\
+    has_treesync_invariants tkt pr
+  )
+  (ensures fun t0 () t1 -> trace_len t1 == trace_len t0 + 2)
+let create #tkt pr p as_session gmgr_session group_id ln secret_session =
+  let now = global_timestamp () in
+  let create_pend = extract_result pr (prepare_create group_id ln) in
+  let token = get_token_for pr p as_session create_pend.as_input in
+  let token: as_token_for (dy_asp pr.global_usage now) create_pend.as_input = token in
+  let st = finalize_create create_pend token in
+  finalize_create_has_pre (is_publishable pr.global_usage now) create_pend token;
+  let si_public = new_public_treesync_state pr p now st in
+  let group_sessions = { si_public; si_private = secret_session; } in
+  add_new_group_sessions pr p gmgr_session group_id group_sessions
+
+val welcome:
+  #tkt:treekem_types dy_bytes ->
+  pr:preds -> p:principal -> as_session:nat -> gmgr_session:nat -> kpmgr_session:nat ->
+  my_key_package:key_package_nt dy_bytes tkt ->
+  group_id:mls_bytes dy_bytes -> l:nat -> t:treesync dy_bytes tkt l 0 ->
+  LCrypto unit pr
+  (requires fun t0 ->
+    is_publishable pr.global_usage (trace_len t0) group_id /\
+    treesync_has_pre (is_publishable pr.global_usage (trace_len t0)) t /\
+    has_treesync_invariants tkt pr
+  )
+  (ensures fun t0 () t1 -> trace_len t1 == trace_len t0 + 2)
+let welcome #tkt pr p as_session gmgr_session kpmgr_session my_key_package group_id l t =
+  let now = global_timestamp () in
+  let welcome_pend = extract_result pr (prepare_welcome group_id t) in
+  welcome_pend.as_inputs_proof;
+  let tokens = get_tokens_for pr p as_session welcome_pend.as_inputs in
+  let tokens: tokens_for_welcome (dy_asp pr.global_usage now) welcome_pend = tokens in
+  let st = finalize_welcome welcome_pend tokens in
+  finalize_welcome_has_pre (is_publishable pr.global_usage now) welcome_pend tokens;
+  let si_public = new_public_treesync_state pr p now st in
+  let si_private = (find_key_package_secret_session tkt pr p kpmgr_session my_key_package).si_private in
+  let group_sessions = { si_public; si_private; } in
+  add_new_group_sessions pr p gmgr_session group_id group_sessions
 
 val add:
   #tkt:treekem_types dy_bytes ->
