fstar/MLS.TreeSync.Symbolic.API.KeyPackageManager.fst
@@ -1,0 +1,50 @@
+module MLS.TreeSync.Symbolic.API.KeyPackageManager
+
+open Comparse
+open MLS.TreeSync.NetworkTypes
+open LabeledRuntimeAPI
+open MLS.Symbolic
+open MLS.Symbolic.MapSession
+open MLS.TreeSync.Symbolic.IsValid
+
+(*** KeyPackage manager types & invariants ***)
+
+type key_package_manager_value (bytes:Type0) {|bytes_like bytes|} = {
+  [@@@ with_parser #bytes ps_nat]
+  si_private: nat;
+}
+
+%splice [ps_key_package_manager_value] (gen_parser (`key_package_manager_value))
+%splice [ps_key_package_manager_value_is_valid] (gen_is_valid_lemma (`key_package_manager_value))
+
+val key_package_manager_types: treekem_types dy_bytes -> map_types dy_bytes
+let key_package_manager_types tkt = {
+  key = key_package_nt dy_bytes tkt;
+  ps_key = ps_key_package_nt tkt;
+  value = key_package_manager_value dy_bytes;
+  ps_value = ps_key_package_manager_value;
+}
+
+val key_package_manager_pred: tkt:treekem_types dy_bytes -> map_predicate (key_package_manager_types tkt)
+let key_package_manager_pred tkt = {
+  pred = (fun gu time (key_package:(key_package_manager_types tkt).key) value ->
+    value_has_pre (is_publishable gu time) key_package
+  );
+  pred_later = (fun gu time0 time1 key_package value ->
+    MLS.MiscLemmas.comparse_is_valid_weaken (ps_key_package_nt tkt) (is_publishable gu time0) (is_publishable gu time1) key_package
+  );
+  pred_is_msg = (fun gu time key_package value -> ());
+}
+
+val key_package_manager_label: string
+let key_package_manager_label = "MLS.TreeSync.KeyPackageManager"
+
+val has_key_package_manager_invariant: treekem_types dy_bytes -> preds -> prop
+let has_key_package_manager_invariant tkt pr =
+  has_map_session_invariant (key_package_manager_types tkt) (key_package_manager_pred tkt) key_package_manager_label pr
+
+(*** KeyPackage manager API ***)
+
+let initialize_key_package_manager (tkt:treekem_types dy_bytes) = initialize_map (key_package_manager_types tkt) (key_package_manager_pred tkt) key_package_manager_label
+let add_new_key_package_secret_session (tkt:treekem_types dy_bytes) = add_key_value (key_package_manager_types tkt) (key_package_manager_pred tkt) key_package_manager_label
+let find_key_package_secret_session (tkt:treekem_types dy_bytes) = find_value (key_package_manager_types tkt) (key_package_manager_pred tkt) key_package_manager_label
